orders.v
@@ -2,11 +2,311 @@
 (* This file is distributed under the terms of the BSD license. *)
 (** This file collects common properties of pre-orders and semi lattices. This
 theory will mainly be used for the theory on collections and finite maps. *)
+Require Export Sorted.
 Require Export base decidable tactics list.
 
-(** * Pre-orders *)
-(** We extend a pre-order to a partial order by defining equality as
-[λ X Y, X ⊆ Y ∧ Y ⊆ X]. We prove that this indeed gives rise to a setoid. *)
+(** * Arbitrary pre-, parial and total orders *)
+(** Properties about arbitrary pre-, partial, and total orders. We do not use
+the relation [⊆] because we often have multiple orders on the same structure *)
+Section orders.
+  Context {A} {R : relation A}.
+  Implicit Types X Y : A.
+
+  Infix "⊆" := R.
+  Notation "X ⊈ Y" := (¬X ⊆ Y).
+  Infix "⊂" := (strict R).
+
+  Lemma reflexive_eq `{!Reflexive R} X Y : X = Y → X ⊆ Y.
+  Proof. by intros <-. Qed.
+  Lemma anti_symmetric_iff `{!PartialOrder R} X Y : X = Y ↔ R X Y ∧ R Y X.
+  Proof. intuition (subst; auto). Qed.
+
+  Lemma strict_spec X Y : X ⊂ Y ↔ X ⊆ Y ∧ Y ⊈ X.
+  Proof. done. Qed.
+  Lemma strict_include X Y : X ⊂ Y → X ⊆ Y.
+  Proof. by intros [? _]. Qed.
+  Lemma strict_ne X Y : X ⊂ Y → X ≠ Y.
+  Proof. by intros [??] <-. Qed.
+  Lemma strict_ne_sym X Y : X ⊂ Y → Y ≠ X.
+  Proof. by intros [??] <-. Qed.
+  Lemma strict_transitive_l `{!Transitive R} X Y Z : X ⊂ Y → Y ⊆ Z → X ⊂ Z.
+  Proof.
+    intros [? HXY] ?. split.
+    * by transitivity Y.
+    * contradict HXY. by transitivity Z.
+  Qed.
+  Lemma strict_transitive_r `{!Transitive R} X Y Z : X ⊆ Y → Y ⊂ Z → X ⊂ Z.
+  Proof.
+    intros ? [? HYZ]. split.
+    * by transitivity Y.
+    * contradict HYZ. by transitivity X.
+  Qed.
+
+  Global Instance: Irreflexive (strict R).
+  Proof. firstorder. Qed.
+  Global Instance: Transitive R → StrictOrder (strict R).
+  Proof.
+    split; try apply _.
+    eauto using strict_transitive_r, strict_include.
+  Qed.
+
+  Global Instance preorder_subset_dec_slow `{∀ X Y, Decision (X ⊆ Y)}
+    (X Y : A) : Decision (X ⊂ Y) | 100 := _.
+
+  Lemma strict_spec_alt `{!PartialOrder R} X Y : X ⊂ Y ↔ X ⊆ Y ∧ X ≠ Y.
+  Proof.
+    split.
+    * intros [? HYX]. split. done. by intros <-.
+    * intros [? HXY]. split. done. by contradict HXY; apply (anti_symmetric R).
+  Qed.
+  Lemma po_eq_dec `{!PartialOrder R} `{∀ X Y, Decision (X ⊆ Y)} (X Y : A) :
+    Decision (X = Y).
+  Proof.
+    refine (cast_if_and (decide (X ⊆ Y)) (decide (Y ⊆ X)));
+     abstract (rewrite anti_symmetric_iff; tauto).
+  Defined.
+
+  Lemma total_not `{!Total R} X Y : X ⊈ Y → Y ⊆ X.
+  Proof. intros. destruct (total R X Y); tauto. Qed.
+  Lemma total_not_strict `{!Total R} X Y : X ⊈ Y → Y ⊂ X.
+  Proof. red; auto using total_not. Qed.
+
+  Global Instance trichotomyT_dec `{!TrichotomyT R} `{!Reflexive R} X Y :
+      Decision (X ⊆ Y) :=
+    match trichotomyT R X Y with
+    | inleft (left H) => left (proj1 H)
+    | inleft (right H) => left (reflexive_eq _ _ H)
+    | inright H => right (proj2 H)
+    end.
+  Global Instance trichotomyT_trichotomy `{!TrichotomyT R} : Trichotomy R.
+  Proof. intros X Y. destruct (trichotomyT R X Y) as [[|]|]; tauto. Qed.
+  Global Instance trichotomy_total `{!Trichotomy R} `{!Reflexive R} : Total R.
+  Proof.
+    intros X Y. destruct (trichotomy R X Y) as [[??]|[<-|[??]]]; intuition.
+  Qed.
+End orders.
+
+Ltac simplify_order := repeat
+  match goal with
+  | _ => progress simplify_equality
+  | H : strict _ ?x ?x |- _ => by destruct (irreflexivity _ _ H)
+  | H1 : ?R ?x ?y |- _ =>
+    match goal with
+    | H2 : R y x |- _ =>
+      assert (x = y) by (by apply (anti_symmetric R)); clear H1 H2
+    | H2 : R y ?z |- _ =>
+      unless (R x z) by done;
+      assert (R x z) by (by transitivity y)
+    end
+  end.
+
+(** * Sorting *)
+(** Merge sort. Adapted from the implementation of Hugo Herbelin in the Coq
+standard library, but without using the module system. *)
+Section merge_sort.
+  Context  {A} (R : relation A) `{∀ x y, Decision (R x y)}.
+
+  Fixpoint list_merge (l1 : list A) : list A → list A :=
+    fix list_merge_aux l2 :=
+    match l1, l2 with
+    | [], _ => l2
+    | _, [] => l1
+    | x1 :: l1, x2 :: l2 =>
+       if decide_rel R x1 x2 then x1 :: list_merge l1 (x2 :: l2)
+       else x2 :: list_merge_aux l2
+    end.
+  Global Arguments list_merge !_ !_ /.
+
+  Local Notation stack := (list (option (list A))).
+  Fixpoint merge_list_to_stack (st : stack) (l : list A) : stack :=
+    match st with
+    | [] => [Some l]
+    | None :: st => Some l :: st
+    | Some l' :: st => None :: merge_list_to_stack st (list_merge l' l)
+    end.
+  Fixpoint merge_stack (st : stack) : list A :=
+    match st with
+    | [] => []
+    | None :: st => merge_stack st
+    | Some l :: st => list_merge l (merge_stack st)
+    end.
+  Fixpoint merge_sort_aux (st : stack) (l : list A) : list A :=
+    match l with
+    | [] => merge_stack st
+    | x :: l => merge_sort_aux (merge_list_to_stack st [x]) l
+    end.
+  Definition merge_sort : list A → list A := merge_sort_aux [].
+End merge_sort.
+
+(** ** Properties of the [Sorted] and [StronglySorted] predicate *)
+Section sorted.
+  Context {A} (R : relation A).
+
+  Lemma Sorted_StronglySorted `{!Transitive R} l :
+    Sorted R l → StronglySorted R l.
+  Proof. by apply Sorted.Sorted_StronglySorted. Qed.
+  Lemma StronglySorted_unique `{!AntiSymmetric (=) R} l1 l2 :
+    StronglySorted R l1 → StronglySorted R l2 → l1 ≡ₚ l2 → l1 = l2.
+  Proof.
+    intros Hl1; revert l2. induction Hl1 as [|x1 l1 ? IH Hx1]; intros l2 Hl2 E.
+    { symmetry. by apply Permutation_nil. }
+    destruct Hl2 as [|x2 l2 ? Hx2].
+    { by apply Permutation_nil in E. }
+    assert (x1 = x2); subst.
+    { rewrite Forall_forall in Hx1, Hx2.
+      assert (x2 ∈ x1 :: l1) as Hx2' by (by rewrite E; left).
+      assert (x1 ∈ x2 :: l2) as Hx1' by (by rewrite <-E; left).
+      inversion Hx1'; inversion Hx2'; simplify_equality; auto. }
+    f_equal. by apply IH, (injective (x2 ::)).
+  Qed.
+  Lemma Sorted_unique `{!Transitive R} `{!AntiSymmetric (=) R} l1 l2 :
+    Sorted R l1 → Sorted R l2 → l1 ≡ₚ l2 → l1 = l2.
+  Proof. auto using StronglySorted_unique, Sorted_StronglySorted. Qed.
+
+  Global Instance HdRel_dec x `{∀ y, Decision (R x y)} l :
+    Decision (HdRel R x l).
+  Proof.
+   refine
+    match l with
+    | [] => left _
+    | y :: l => cast_if (decide (R x y))
+    end; abstract first [by constructor | by inversion 1].
+  Defined.
+
+  Global Instance Sorted_dec `{∀ x y, Decision (R x y)} : ∀ l,
+    Decision (Sorted R l).
+  Proof.
+   refine
+    (fix go l :=
+    match l return Decision (Sorted R l) with
+    | [] => left _
+    | x :: l => cast_if_and (decide (HdRel R x l)) (go l)
+    end); clear go; abstract first [by constructor | by inversion 1].
+  Defined.
+  Global Instance StronglySorted_dec `{∀ x y, Decision (R x y)} : ∀ l,
+    Decision (StronglySorted R l).
+  Proof.
+   refine
+    (fix go l :=
+    match l return Decision (StronglySorted R l) with
+    | [] => left _
+    | x :: l => cast_if_and (decide (Forall (R x) l)) (go l)
+    end); clear go; abstract first [by constructor | by inversion 1].
+  Defined.
+
+  Context {B} (f : A → B).
+  Lemma HdRel_fmap (R1 : relation A) (R2 : relation B) x l :
+    (∀ y, R1 x y → R2 (f x) (f y)) → HdRel R1 x l → HdRel R2 (f x) (f <$> l).
+  Proof. destruct 2; constructor; auto. Qed.
+  Lemma Sorted_fmap (R1 : relation A) (R2 : relation B) l :
+    (∀ x y, R1 x y → R2 (f x) (f y)) → Sorted R1 l → Sorted R2 (f <$> l).
+  Proof. induction 2; simpl; constructor; eauto using HdRel_fmap. Qed.
+  Lemma StronglySorted_fmap (R1 : relation A) (R2 : relation B) l :
+    (∀ x y, R1 x y → R2 (f x) (f y)) →
+    StronglySorted R1 l → StronglySorted R2 (f <$> l).
+  Proof.
+    induction 2; simpl; constructor;
+      rewrite ?Forall_fmap; eauto using Forall_impl.
+  Qed.
+End sorted.
+
+(** ** Correctness of merge sort *)
+Section merge_sort_correct.
+  Context  {A} (R : relation A) `{∀ x y, Decision (R x y)} `{!Total R}.
+
+  Lemma list_merge_cons x1 x2 l1 l2 :
+    list_merge R (x1 :: l1) (x2 :: l2) =
+      if decide (R x1 x2) then x1 :: list_merge R l1 (x2 :: l2)
+      else x2 :: list_merge R (x1 :: l1) l2.
+  Proof. done. Qed.
+
+  Lemma HdRel_list_merge x l1 l2 :
+    HdRel R x l1 → HdRel R x l2 → HdRel R x (list_merge R l1 l2).
+  Proof.
+    destruct 1 as [|x1 l1 IH1], 1 as [|x2 l2 IH2];
+      rewrite ?list_merge_cons; simpl; repeat case_decide; auto.
+  Qed.
+  Lemma Sorted_list_merge l1 l2 :
+    Sorted R l1 → Sorted R l2 → Sorted R (list_merge R l1 l2).
+  Proof.
+    intros Hl1. revert l2. induction Hl1 as [|x1 l1 IH1];
+      induction 1 as [|x2 l2 IH2]; rewrite ?list_merge_cons; simpl;
+      repeat case_decide;
+      constructor; eauto using HdRel_list_merge, HdRel_cons, total_not.
+  Qed.
+  Lemma merge_Permutation l1 l2 : list_merge R l1 l2 ≡ₚ l1 ++ l2.
+  Proof.
+    revert l2. induction l1 as [|x1 l1 IH1]; intros l2;
+      induction l2 as [|x2 l2 IH2]; rewrite ?list_merge_cons; simpl;
+      repeat case_decide; auto.
+    * by rewrite (right_id_L [] (++)).
+    * by rewrite IH2, Permutation_middle.
+  Qed.
+
+  Local Notation stack := (list (option (list A))).
+  Inductive merge_stack_Sorted : stack → Prop :=
+    | merge_stack_Sorted_nil : merge_stack_Sorted []
+    | merge_stack_Sorted_cons_None st :
+       merge_stack_Sorted st → merge_stack_Sorted (None :: st)
+    | merge_stack_Sorted_cons_Some l st :
+       Sorted R l → merge_stack_Sorted st → merge_stack_Sorted (Some l :: st).
+  Fixpoint merge_stack_flatten (st : stack) : list A :=
+    match st with
+    | [] => []
+    | None :: st => merge_stack_flatten st
+    | Some l :: st => l ++ merge_stack_flatten st
+    end.
+
+  Lemma Sorted_merge_list_to_stack st l :
+    merge_stack_Sorted st → Sorted R l →
+    merge_stack_Sorted (merge_list_to_stack R st l).
+  Proof.
+    intros Hst. revert l.
+    induction Hst; repeat constructor; naive_solver auto using Sorted_list_merge.
+  Qed.
+  Lemma merge_list_to_stack_Permutation st l :
+    merge_stack_flatten (merge_list_to_stack R st l) ≡ₚ
+      l ++ merge_stack_flatten st.
+  Proof.
+    revert l. induction st as [|[l'|] st IH]; intros l; simpl; auto.
+    by rewrite IH, merge_Permutation, (associative_L _), (commutative (++) l).
+  Qed.
+  Lemma Sorted_merge_stack st :
+    merge_stack_Sorted st → Sorted R (merge_stack R st).
+  Proof. induction 1; simpl; auto using Sorted_list_merge. Qed.
+  Lemma merge_stack_Permutation st : merge_stack R st ≡ₚ merge_stack_flatten st.
+  Proof.
+    induction st as [|[] ? IH]; intros; simpl; auto.
+    by rewrite merge_Permutation, IH.
+  Qed.
+  Lemma Sorted_merge_sort_aux st l :
+    merge_stack_Sorted st → Sorted R (merge_sort_aux R st l).
+  Proof.
+    revert st. induction l; simpl;
+      auto using Sorted_merge_stack, Sorted_merge_list_to_stack.
+  Qed.
+  Lemma merge_sort_aux_Permutation st l :
+    merge_sort_aux R st l ≡ₚ merge_stack_flatten st ++ l.
+  Proof.
+    revert st. induction l as [|?? IH]; simpl; intros.
+    * by rewrite (right_id_L [] (++)), merge_stack_Permutation.
+    * rewrite IH, merge_list_to_stack_Permutation; simpl.
+      by rewrite Permutation_middle.
+  Qed.
+
+  Lemma Sorted_merge_sort l : Sorted R (merge_sort R l).
+  Proof. apply Sorted_merge_sort_aux. by constructor. Qed.
+  Lemma merge_sort_Permutation l : merge_sort R l ≡ₚ l.
+  Proof. unfold merge_sort. by rewrite merge_sort_aux_Permutation. Qed.
+  Lemma StronglySorted_merge_sort `{!Transitive R} l :
+    StronglySorted R (merge_sort R l).
+  Proof. auto using Sorted_StronglySorted, Sorted_merge_sort. Qed.
+End merge_sort_correct.
+
+(** * Canonical pre and partial orders *)
+(** We extend the canonical pre-order [⊆] to a partial order by defining setoid
+equality as [λ X Y, X ⊆ Y ∧ Y ⊆ X]. We prove that this indeed gives rise to a
+setoid. *)
 Section preorder.
   Context `{SubsetEq A} `{!PreOrder (⊆)}.
 
@@ -27,45 +327,18 @@ Section preorder.
     * transitivity y1. tauto. transitivity y2; tauto.
   Qed.
 
-  Global Instance preorder_subset: Subset A := λ X Y, X ⊆ Y ∧ Y ⊈ X.
-  Lemma subset_spec X Y : X ⊂ Y ↔ X ⊆ Y ∧ Y ⊈ X.
-  Proof. done. Qed.
-  Lemma subset_spec_alt X Y : X ⊂ Y ↔ X ⊆ Y ∧ X ≢ Y.
+  Lemma subset_spec X Y : X ⊂ Y ↔ X ⊆ Y ∧ X ≢ Y.
   Proof.
     split.
     * intros [? HYX]. split. done. contradict HYX. by rewrite HYX.
     * intros [? HXY]. split. done. by contradict HXY.
   Qed.
 
-  Lemma subset_subseteq X Y : X ⊂ Y → X ⊆ Y.
-  Proof. by intros [? _]. Qed.
-  Lemma subset_transitive_l X Y Z : X ⊂ Y → Y ⊆ Z → X ⊂ Z.
-  Proof.
-    intros [? HXY] ?. split.
-    * by transitivity Y.
-    * contradict HXY. by transitivity Z.
-  Qed.
-  Lemma subset_transitive_r X Y Z : X ⊆ Y → Y ⊂ Z → X ⊂ Z.
-  Proof.
-    intros ? [? HYZ]. split.
-    * by transitivity Y.
-    * contradict HYZ. by transitivity X.
-  Qed.
-
-  Global Instance: StrictOrder (⊂).
-  Proof.
-    split.
-    * firstorder.
-    * eauto using subset_transitive_r, subset_subseteq.
-  Qed.
-  Global Instance: Proper ((≡) ==> (≡) ==> iff) (⊂).
-  Proof. unfold subset, preorder_subset. solve_proper. Qed.
-
   Section leibniz.
     Context `{!LeibnizEquiv A}.
 
-    Lemma subset_spec_alt_L X Y : X ⊂ Y ↔ X ⊆ Y ∧ X ≠ Y.
-    Proof. unfold_leibniz. apply subset_spec_alt. Qed.
+    Lemma subset_spec_L X Y : X ⊂ Y ↔ X ⊆ Y ∧ X ≠ Y.
+    Proof. unfold_leibniz. apply subset_spec. Qed.
   End leibniz.
 
   Section dec.
@@ -73,13 +346,11 @@ Section preorder.
 
     Global Instance preorder_equiv_dec_slow (X Y : A) :
       Decision (X ≡ Y) | 100 := _.
-    Global Instance preorder_subset_dec_slow (X Y : A) :
-      Decision (X ⊂ Y) | 100 := _.
 
     Lemma subseteq_inv X Y : X ⊆ Y → X ⊂ Y ∨ X ≡ Y.
-    Proof. rewrite subset_spec_alt. destruct (decide (X ≡ Y)); tauto. Qed.
+    Proof. rewrite subset_spec. destruct (decide (X ≡ Y)); tauto. Qed.
     Lemma not_subset_inv X Y : X ⊄ Y → X ⊈ Y ∨ X ≡ Y.
-    Proof. rewrite subset_spec_alt. destruct (decide (X ≡ Y)); tauto. Qed.
+    Proof. rewrite subset_spec. destruct (decide (X ≡ Y)); tauto. Qed.
 
     Context `{!LeibnizEquiv A}.
 
@@ -91,7 +362,6 @@ Section preorder.
 End preorder.
 
 Typeclasses Opaque preorder_equiv.
-Typeclasses Opaque preorder_subset.
 Hint Extern 0 (@Equivalence _ (≡)) =>
   class_apply preorder_equivalence : typeclass_instances.
 
@@ -102,7 +372,7 @@ Section partialorder.
   Global Instance: LeibnizEquiv A.
   Proof.
     split.
-    * intros [??]. by apply (anti_symmetric _).
+    * intros [??]. by apply (anti_symmetric (⊆)).
     * intros. by subst.
   Qed.
 End partialorder.
@@ -337,7 +607,6 @@ Section lower_bounded_lattice.
   Qed.
   Global Instance: RightAbsorb (≡) ∅ (∩).
   Proof. intros ?. by rewrite (commutative _), (left_absorb _ _). Qed.
-
   Global Instance: LeftDistr (≡) (∪) (∩).
   Proof.
     intros x y z. split.
@@ -350,7 +619,6 @@ Section lower_bounded_lattice.
   Qed.
   Global Instance: RightDistr (≡) (∪) (∩).
   Proof. intros x y z. by rewrite !(commutative _ _ z), (left_distr _ _). Qed.
-
   Global Instance: LeftDistr (≡) (∩) (∪).
   Proof.
     intros x y z. split.
@@ -378,12 +646,10 @@ Section lower_bounded_lattice.
     Proof. intros ?. unfold_leibniz. apply (left_absorb _ _). Qed.
     Global Instance: RightAbsorb (=) ∅ (∩).
     Proof. intros ?. unfold_leibniz. apply (right_absorb _ _). Qed.
-
     Global Instance: LeftDistr (=) (∪) (∩).
     Proof. intros ???. unfold_leibniz. apply (left_distr _ _). Qed.
     Global Instance: RightDistr (=) (∪) (∩).
     Proof. intros ???. unfold_leibniz. apply (right_distr _ _). Qed.
-
     Global Instance: LeftDistr (=) (∩) (∪).
     Proof. intros ???. unfold_leibniz. apply (left_distr _ _). Qed.
     Global Instance: RightDistr (=) (∩) (∪).
